---
layout: default
title: Asymmetric FGM copula
---

# Asymmetric FGM copula

cdf
---

Following [[Nel06]](#refs), with $$b=0$$:

$$C(u_{1},u_{2})=u_{1}u_{2} + \theta u_{1}u_{2}(1 - u_{1} - u_{2} +
u_{1}u_{2})u_{2}(1 - u_{1})$$ 

pdf 
----
[[Wolfram|Alpha]](http://www.wolframalpha.com/share/clip?f=d41d8cd98f00b204e9800998ecf8427eq5ppn2koc6)

$$c(u_{1},u_{2})= u_{1} \left( \theta u_{1} (6-9 u_{2})u_{2} +
\theta(12 u_{2}-8)u_{2} \right) + \theta(2-3 u_{2})u_{2} +1 $$

hfun 
----
[[Wolfram|Alpha]](http://www.wolframalpha.com/share/clip?f=d41d8cd98f00b204e9800998ecf8427e7tgb7ub1or)

$$h(u_{1},u_{2})=-3\theta u_{1}^{3}u_{2}^{2}+ 2\theta u_{1}^{3}u_{2} + 6\theta
u_{1}^{2}u_{2}^{2}-4\theta u_{1}^{2}u_{2} - 3\theta u_{1}u_{2}^{2} +
2\theta u_{1}u_{2} + u_{1}$$

vfun 
----
[[Wolfram|Alpha]](http://www.wolframalpha.com/share/clip?f=d41d8cd98f00b204e9800998ecf8427efrq94pkrfc)

$$v(u_{2},u_{1})= -3\theta u_{1}^{2}u_{2}^{3} + 3\theta
u_{1}^{2}u_{2}^{2} + 4\theta u_{1}u_{2}^{3} - 4 \theta
u_{1}u_{2}^{2} - \theta u_{2}^{3} + \theta u_{2}^{2} + u_{2}$$



References<a name="refs"></a>
---------

<iframe src="../refs/html_refs/asym_fgm.html" width="600" height="200"></iframe>
